specs/Address.v
@@ -1,22 +1,26 @@
 Require Import FreeSpec.Specs.Memory.
 Require Import Coq.Init.Nat.
+Require Import Coq.NArith.NArith.
 
 (* we only consider 32 bit system *)
 Definition address := lword.
 
+Local Close Scope nat_scope.
+Local Open Scope N_scope.
+
 Definition is_pow_2
-           (n: nat)
+           (n:  N)
   : Prop :=
-  2 ^ (Nat.log2 n) = n.
+  2 ^ (N.log2 n) = n.
 
 Program Definition is_aligned
-        (x:    address)
-        (base: nat | is_pow_2 base)
+        (x:     address)
+        (base:  N | is_pow_2 base)
   : Prop :=
   cast base x = box base 0.
 
 Program Definition aligned_address
-        (n: nat | is_pow_2 n)
+        (n:  N | is_pow_2 n)
   : Type :=
   {addr: address | is_aligned addr n}.
 
